wip

src/matroid/minor.lean
@@ -12,29 +12,29 @@ variables {U : ftype}
 /-- a matroid_in U corresponds to a matroid defined on some subset E of U. Implemented as a matroid on which the nonelements of 
 E are all loops. -/
 @[ext] structure matroid_in (U : ftype) :=
-(groundset : set U)
+(E : set U)
 (carrier : matroid U)
-(support : carrier.r groundsetᶜ = 0)
+(support : carrier.r Eᶜ = 0)
 
 namespace matroid_in 
 
-/-- the rank of a set X wrt a matroid_in U. Elements of X outside the groundset of U are ignored -/
+/-- the rank of a set X wrt a matroid_in U. Elements of X outside the E of U are ignored -/
 def r (M : matroid_in U)(X : set U) := M.carrier.r X 
 
-lemma ext' (M₁ M₂ : matroid_in U)(h_ground : M₁.groundset = M₂.groundset)(h_r : ∀ X ⊆ M₁.groundset, M₁.r X = M₂.r X):
+lemma ext' {M₁ M₂ : matroid_in U}(h_ground : M₁.E = M₂.E)(h_r : ∀ X ⊆ M₁.E, M₁.r X = M₂.r X):
   M₁ = M₂ := 
 begin
   apply matroid_in.ext _ _ h_ground, ext X,
-  specialize h_r (X ∩ M₁.groundset) (by simp),  
-  rw (by simp : X = (X ∩ M₁.groundset) ∪ (X ∩ M₁.groundsetᶜ)), 
+  specialize h_r (X ∩ M₁.E) (by simp),  
+  rw (by simp : X = (X ∩ M₁.E) ∪ (X ∩ M₁.Eᶜ)), 
   have h₁ := matroid.rank_inter_rank_zero X M₁.support,
   have h₂ := matroid.rank_inter_rank_zero X M₂.support, rw ←h_ground at h₂, 
-  rw [matroid.rank_eq_rank_union_rank_zero (X ∩ M₁.groundset) h₁, matroid.rank_eq_rank_union_rank_zero (X ∩ M₁.groundset) h₂], 
+  rw [matroid.rank_eq_rank_union_rank_zero (X ∩ M₁.E) h₁, matroid.rank_eq_rank_union_rank_zero (X ∩ M₁.E) h₂], 
   exact h_r, 
 end
 
-/-- the ftype coming from the groundset of M -/
-def ground (M : matroid_in U) := subftype M.groundset
+/-- the ftype coming from the E of M -/
+def ground (M : matroid_in U) := subftype M.E
 
 /-- a matroid_in U gives a matroid on a subtype -/
 def as_mat_on (M : matroid_in U)(E : set U) : matroid (subftype E) := 
@@ -44,10 +44,13 @@ def as_mat_on (M : matroid_in U)(E : set U) : matroid (subftype E) :=
   R2 := λ X Y hXY, by {apply M.carrier.R2, apply set.image_subset _ hXY, },
   R3 := λ X Y, by {dsimp only, convert M.carrier.R3 _ _, apply set.image_union, exact (set.image_inter subtype.val_injective).symm} }
 
-/-- a matroid_in U, viewed as a matroid on the subtype defined by its groundset -/
-def as_mat (M : matroid_in U) : matroid M.ground := as_mat_on M M.groundset 
+/-- a matroid_in U, viewed as a matroid on the subtype defined by its E -/
+def as_mat (M : matroid_in U) : matroid M.ground := as_mat_on M M.E 
 
-@[simp] lemma as_mat_r (M : matroid_in U)(X : set (subftype M.groundset)): 
+mk_simp_attribute msimp "minor simp lemmas"
+
+
+@[simp, msimp] lemma as_mat_r (M : matroid_in U)(X : set (subftype M.E)): 
   M.as_mat.r X = M.r (X : set U) :=
 rfl 
 
@@ -55,7 +58,7 @@ rfl
 
 /-- a matroid_in U, constructed from a matroid on a subtype of U -/
 def of_mat {E : set U}(N : matroid (subftype E)) : matroid_in U := 
-{ groundset := E,
+{ E := E,
   carrier := 
   { r := λ X, N.r (inter_subtype E X ),
     R0 := λ X, N.R0 _,
@@ -64,12 +67,29 @@ def of_mat {E : set U}(N : matroid (subftype E)) : matroid_in U :=
     R3 := λ X Y, N.R3 _ _, },
   support := by {simp [inter_subtype],} }
 
-@[simp] lemma of_mat_groundset {E : set U}(N : matroid (subftype E)) : (of_mat N).groundset = E := rfl 
+@[simp, msimp] lemma of_mat_E {E : set U}(N : matroid (subftype E)) : 
+  (of_mat N).E = E :=
+rfl 
 
-@[simp] lemma of_mat_r {E : set U}(N : matroid (subftype E))(X : set U) : (of_mat N).r X = N.r (inter_subtype E X) := rfl 
+@[simp, msimp] lemma of_mat_r {E : set U}(N : matroid (subftype E))(X : set U) : 
+  (of_mat N).r X = N.r (inter_subtype E X) := 
+rfl 
+
+lemma r_of_mat {E : set U}(N : matroid (subftype E))(X : set (subftype E)): 
+  N.r X = (of_mat N).r X := 
+begin
+  simp only [matroid_in.of_mat_r], convert rfl, 
+  unfold inter_subtype, ext x , --rcases x with ⟨x,hx⟩, 
+  simp only [set.mem_set_of_eq, subtype.coe_mk], 
+  refine ⟨λ h, _, λ h, ⟨x,⟨h, by simp⟩⟩ ⟩,
+  rcases h with ⟨⟨y, h⟩, h', h''⟩, 
+  cases x, 
+  simp only [subtype.coe_mk] at h'', 
+  convert h',  rwa h'', 
+end
 
 
-lemma as_mat_of_mat {E : set U}(N : matroid (subftype E)) : 
+@[simp,msimp] lemma as_mat_of_mat {E : set U}(N : matroid (subftype E)) : 
   as_mat (of_mat N) = N :=
 begin
   ext X, dsimp only [as_mat, as_mat_on, of_mat], convert rfl, ext x, 
@@ -78,6 +98,12 @@ begin
   refine ⟨λ h, by {cases x, tauto}, λ h, _⟩,
   cases x with x hx, rcases h with ⟨y,z, h⟩, convert h.1, convert h.2.symm, 
 end
+
+@[simp,msimp] lemma of_mat_as_mat (M : matroid_in U) : 
+  of_mat (as_mat M) = M :=
+ext' (by simp) 
+     (λ X hX, by {simp only with msimp coe_up at *, convert rfl, rw subset_def_inter_mp hX}) 
+
 
 lemma of_mat_as_mat_on {E E' : set U}(N : matroid (subftype E))(h : E' = E): 
    of_mat ((of_mat N).as_mat_on E') = of_mat N := 
@@ -95,17 +121,54 @@ begin
   rw h, exact ⟨⟨e,he⟩,⟨h',rfl⟩⟩,
 end
 
+lemma of_mat_inj {R : set U}(N N' : matroid (subftype R)):
+  of_mat N = of_mat N' → N = N' := 
+λ h, by {ext, rw [r_of_mat,r_of_mat,h]}  
 
 def as_matroid_in (M : matroid U) : matroid_in U := ⟨univ, M, by simp⟩
 
 instance coe_to_matroid_in : has_coe (matroid U) (matroid_in U) := ⟨λ M, as_matroid_in M⟩
 
+
+
+
+def dual (M : matroid_in U) : matroid_in U := 
+  of_mat (as_mat M).dual 
+
+@[simp, msimp] lemma dual_r (M : matroid_in U)(X : set U) :
+  (dual M).r X = size (X ∩ M.E) + M.r (M.E \ X) - M.r M.E  :=
+begin
+  rw [dual, of_mat_r, matroid.dual_r], simp only with coe_up, convert rfl, 
+  simp only with coe_up, 
+  ext,simp only [ftype.diff_def, set.mem_inter_eq, set.mem_compl_eq], tauto, 
+  simp only with coe_up, 
+end 
+
+lemma of_mat_dual {E : set U}(M : matroid (subftype E)): 
+  of_mat M.dual = (of_mat M).dual := 
+by {unfold dual, convert rfl, simp}
+
+
+@[simp, msimp] lemma dual_ground (M : matroid_in U): 
+  (dual M).E = M.E := 
+rfl 
+
+@[simp, msimp] lemma dual_dual (M : matroid_in U):
+  M.dual.dual = M := 
+by {simp_rw [dual,of_mat_dual, as_mat_of_mat, ←of_mat_dual, matroid.dual_dual, of_mat_as_mat]}
+
+lemma dual_inj {M M' : matroid_in U}(h : M.dual = M'.dual):
+  M = M' := 
+by rw [←dual_dual M, ←dual_dual M',h]
+
+
+
 section minor 
 
 /-- minor relation between two matroid_in U-/
 def is_minor (N M : matroid_in U) : Prop := 
-  (N.groundset ⊆ M.groundset) ∧ 
-  ∃ C ⊆ M.groundset \ N.groundset, (∀ X ⊆ N.groundset, N.r X = M.r (X ∪ C) - M.r C)  
+  (N.E ⊆ M.E) ∧ 
+  ∃ C ⊆ M.E \ N.E, (∀ X ⊆ N.E, N.r X = M.r (X ∪ C) - M.r C)  
 
 /-- minor relation between a matroid_in U and a matroid U -/
 def is_minor_of (N : matroid_in U)(M : matroid U) := 
@@ -119,36 +182,35 @@ begin
     simp only [ftype.diff_def, set.mem_inter_eq, set.mem_union_eq, set.mem_compl_eq], 
     tauto, },
   -- set_solver should work for the goal above, but it is glacial
-  have hC₁M₂: C₁ ⊆ M₂.groundset := by 
+  have hC₁M₂: C₁ ⊆ M₂.E := by 
   { intros x hx, simp only [ftype.diff_def, set.subset_inter_iff] at hC₁, tauto,},
   rw [h1' X hX, h2' (X ∪ C₁) _, h2' C₁ hC₁M₂, ←union_assoc],  ring,
   exact union_is_ub (subset_trans hX h1) hC₁M₂, 
 end 
-
 def contract (M : matroid_in U)(C : set U) : matroid_in U := 
-⟨ M.groundset \ C, 
+⟨ M.E \ C, 
   M.carrier.project C, 
   by {convert M.carrier.projected_set_union_rank_zero C M.support, set_solver}⟩
 
-@[simp] lemma contract_rank (M : matroid_in U)(C X: set U): 
+@[simp, msimp] lemma contract_rank (M : matroid_in U)(C X: set U): 
   (M.contract C).r X = M.r (X ∪ C) - M.r C :=
 M.carrier.project_r _ _ 
 
-@[simp] lemma contract_groundset (M : matroid_in U)(C: set U):
-  (M.contract C).groundset = M.groundset \ C := 
+@[simp, msimp] lemma contract_E (M : matroid_in U)(C: set U):
+  (M.contract C).E = M.E \ C := 
 rfl 
 
 def delete (M : matroid_in U)(D : set U) : matroid_in U := 
-⟨ M.groundset \ D, 
+⟨ M.E \ D, 
   M.carrier.loopify D, 
   by {convert M.carrier.loopified_set_union_rank_zero D M.support, set_solver,}⟩
 
-@[simp] lemma delete_rank (M : matroid_in U)(D X: set U): 
+@[simp, msimp] lemma delete_rank (M : matroid_in U)(D X: set U): 
   (M.delete D).r X = M.r (X \ D) :=
 rfl
 
-@[simp] lemma delete_groundset (M : matroid_in U)(D: set U):
-  (M.delete D).groundset = M.groundset \ D := 
+@[simp, msimp] lemma delete_E (M : matroid_in U)(D: set U):
+  (M.delete D).E = M.E \ D := 
 rfl 
 
 lemma con_del_eq_del_con (M : matroid_in U)(C D : set U)(h : C ∩ D = ∅) : 
@@ -161,22 +223,101 @@ begin
   set_solver,
 end
 
-
-lemma dual_con_eq_del_dual (M : matroid_in U)(A : set U)(hA : A ⊆ M.groundset): 
+lemma dual_con_eq_del_dual (M : matroid_in U)(A : set U)(hA : A ⊆ M.E): 
   of_mat ((M.contract A).as_mat.dual) = (of_mat M.as_mat.dual).delete A :=
 begin
-  refine ext' _ _ (by simp) (λ X hX, _),
-  
-  simp only [ftype.diff_def, delete_rank, of_mat_r, matroid.dual_r, contract_groundset,
-  contract_rank, as_mat_r] with coe_up, 
-
-
-  simp only [ftype.diff_def, matroid_in.contract_groundset, set.subset_inter_iff, matroid_in.of_mat_groundset] at hX, 
-  
-  rw (λ p q r z, by ring : ∀ p q r z : ℤ, p + (q-z) - (r-z) = p + q - r), 
-  rw [inter_comm _ Aᶜ, ←inter_assoc], 
+  refine ext' (by simp) (λ X hX, _),
+  simp only [matroid.dual_r, ftype.diff_def] with msimp coe_up, 
+  rw [(λ p q r z, by ring : ∀ p q r z : ℤ, p + (q-z) - (r-z) = p + q - r), 
+  inter_comm _ Aᶜ, ←inter_assoc], 
   convert rfl; { ext, simp, tauto},
 end
+
+
+lemma dual_con (M : matroid_in U)(A : set U)(hu : A ⊆ M.E): 
+  (M.contract A).dual = (M.dual).delete A :=
+begin
+  refine ext' (by simp) (λ X hX, _),
+  simp only [matroid.dual_r, ftype.diff_def] with msimp coe_up, 
+  rw [(λ p q r z, by ring : ∀ p q r z : ℤ, p + (q-z) - (r-z) = p + q - r), 
+  inter_comm _ Aᶜ, ←inter_assoc], 
+  convert rfl; { ext, simp, tauto},
+end
+
+lemma dual_del (M : matroid_in U)(A : set U)(hu : A ⊆ M.E): 
+  (M.delete A).dual = (M.dual).contract A :=
+by {rw [←dual_dual M, ← dual_con, dual_dual, dual_dual], exact hu}
+
+lemma dual_con_del (M : matroid_in U)(C D : set U)(hi : C ∩ D = ∅)(hu : C ∪ D ⊆ M.E): 
+  ((M.contract C).delete D).dual = ((M.dual).contract D).delete C :=
+begin
+  have : D ⊆ (M.contract C).E := by {simp only with msimp, set_solver, }, 
+  rw dual_del _ D this, 
+  
+
+
+end
+
+lemma minor_has_delete_contract {M N : matroid_in U}(h : is_minor N M): 
+ ∃ C D, C ∪ D = M.E \ N.E ∧ C ∩ D = ∅ ∧ N = (M.contract C).delete D := 
+begin
+  rcases h with ⟨h, C, hC, hr⟩, 
+  refine ⟨C, (M.E \ N.E) \ C, by { ext, simp at *, tauto,}, by simp, _⟩, 
+  refine ext' (by { ext, simp at *, tauto,}) (λ X hX, _), 
+  rw hr X hX, 
+  simp only [ftype.diff_def, matroid_in.contract_rank, matroid_in.delete_rank, sub_left_inj], 
+  convert rfl, 
+  ext, simp, tauto, 
+end
+
+lemma minor_iff_has_delete_contract {M N : matroid_in U} : 
+  is_minor N M 
+↔ ∃ C D, C ∪ D = M.E \ N.E ∧ C ∩ D = ∅ ∧ N = (M.contract C).delete D :=
+begin
+  split, apply minor_has_delete_contract, 
+  rintros ⟨C ,D, hu, hi, rfl⟩, 
+  refine ⟨_,⟨C,_,_⟩⟩, 
+  { intros x hx, simp at *, tauto, },
+  simp only [ftype.diff_def] with msimp at *,  
+  {apply inter_is_lb, 
+    { refine subset_trans (subset_union_left C D) _, rw hu, apply inter_subset_left,   },
+  intros x hx, simp, tauto, },
+  intros X hX, 
+  simp only with msimp at *, convert rfl,
+  ext, simp at *, tauto,  
+end
+
+def minor_pair {M N : matroid_in U}(h : is_minor N M) : Type := 
+  {p : set U × set U // 
+    p.1 ∩ p.2 = ∅ 
+  ∧ p.1 ∪ p.2 = M.E \ N.E
+  ∧ N = ((M: matroid_in U).contract p.1).delete p.2} 
+
+instance minor_pair_nonempty {M N : matroid_in U}(h : is_minor N M) :
+  nonempty (minor_pair h):= 
+begin
+  apply nonempty_subtype.mpr, 
+  rcases minor_has_delete_contract h with ⟨C,D, h', h'', rfl⟩,
+  refine ⟨⟨C,D⟩, _,_,by simp⟩; try {assumption}, 
+end
+
+instance minor_pair_fintype {M N : matroid_in U}(h : is_minor N M) :
+  fintype (minor_pair h):=  
+by {unfold minor_pair, apply_instance}
+
+
+lemma minor_has_good_delete_contract {M : matroid U}{N : matroid_in U}:
+  is_minor N M → ∃ (C D : set U), 
+  C ∩ D = ∅ 
+  ∧ N = ((M : matroid_in U).contract C).delete D 
+  ∧ M.is_indep C ∧ M.dual.is_indep D   :=
+begin
+  intro h_minor, 
+  set badness : minor_pair h_minor → ℤ := 
+  
+end
+
+
 
 end minor 
 
